theories/TM/Code/BinNumbers/PosMultTM.v
@@ -36,7 +36,7 @@ Check eq_refl : let x := 43 in let y := 24 in mult_TR x y = x * y.
 
 
 (* (* NB: Haskell extraction is fun! *)
-From Coq Require Extraction.
+From Coq From Undecidability Require Extraction.
 Extraction Language Haskell.
 Recursive Extraction mult_TR Pos.mul.
 *)
@@ -229,7 +229,7 @@ Definition Mult_Rel : pRel sigPos^+ unit 3 :=
     forall (x y : positive),
       tin[@Fin0] ≃ x ->
       tin[@Fin1] ≃ y ->
-      isRight tin[@Fin2] ->
+      isVoid tin[@Fin2] ->
       tout[@Fin0] ≃ x /\
       tout[@Fin1] ≃ y /\
       tout[@Fin2] ≃ x*y.
