theories/TM/Combinators/SequentialComposition.v
@@ -39,6 +39,19 @@ Section Composition.
     - intros tin i (i1&i2&Hi&HT1&HT2). exists i1, i2; repeat split; auto.
   Qed.
 
+  (** Strong version *)
+  Lemma Seq_TerminatesIn' R1 T1 T2 :
+    pM1 ⊨ R1 ->
+    projT1 pM1 ↓ T1 ->
+    projT1 pM2 ↓ T2 ->
+    projT1 Seq ↓ (fun tin i => exists i1, T1 tin i1 /\ forall tout yout, R1 tin (yout, tout) -> exists i2, 1 + i1 + i2 <= i /\ T2 tout i2).
+  Proof.
+    intros HRealise HTerm1 HTerm2.
+    eapply TerminatesIn_monotone.
+    - eapply Switch_TerminatesIn'; eauto. instantiate (1 := fun _ => T2). auto.
+    - intros tin i (i1&HT1&H). exists i1; repeat split; eauto.
+  Qed.
+
 
   Lemma Seq_RealiseIn (R1 : Rel _ _) (R2 : Rel _ (F2 * _)) k1 k2:
     pM1 ⊨c(k1) R1 ->
