theories/TM/Hoare/Hoare.v
@@ -1,0 +1,13 @@
+(** * A New Logic  for the specification of Turing Machines, Based on Hoare Logic *)
+
+From Undecidability Require Export TM.Hoare.HoareLogic. (** Abstract definition of Hoare triples *)
+From Undecidability Require Export TM.Hoare.HoareCombinators. (** Rules for the combinators *)
+From Undecidability Require Export TM.Hoare.HoareRegister. (** Definition of a specification language for Register machines; rules for lifts *)
+From Undecidability Require Export TM.Hoare.HoareTactics. (** Verification step tactics *)
+From Undecidability Require Export TM.Hoare.HoareStdLib. (** Hoare rules for standard machine *)
+
+
+(* TODO:
+- Prefix "_size" or "_space"?
+- Univ
+*)
