theories/TM/Hoare/HoareExamples.v
@@ -1,0 +1,1022 @@
+(** ** Examples *)
+
+From Undecidability Require Import ProgrammingTools.
+From Undecidability Require Import Hoare.HoareLogic Hoare.HoareCombinators Hoare.HoareRegister Hoare.HoareTactics.
+From Undecidability Require Import CaseNat.
+
+From Coq Require Import ArithRing. (* for [ring_simplify] *)
+
+Arguments mult : simpl never.
+Arguments plus : simpl never.
+
+
+(* Disable the warnings regarding [Undo]. This is a demonstration file. *)
+Set Warnings "-undo-batch-mode,-non-interactive".
+
+
+(** *** Copy.v *)
+
+From Undecidability Require Import TM.Code.Copy.
+
+Definition CopyValue_sizefun {sigX X : Type} {cX : codable sigX X} (x : X) : Vector.t (nat->nat) 2 := [|id; CopyValue_size x|].
+
+(** This is how we specify partital correctness, time, and space in one lemma *)
+Lemma CopyValue_SpecT_size (sig : finType) (sigX X : Type) (cX : codable sigX X) (I : Retract sigX sig) (x : X) (ss : Vector.t nat 2) :
+  TripleT (tspec (withSpace (SpecVector [|Contains _ x; Void|]) ss))
+          (CopyValue_steps x) (CopyValue _)
+          (fun _ => tspec (withSpace (SpecVector [|Contains _ x; Contains _ x|]) (appSize (CopyValue_sizefun x) ss))).
+Proof.
+  eapply Realise_TripleT.
+  - apply CopyValue_Realise.
+  - apply CopyValue_Terminates.
+  - intros tin [] tout H HEnc. cbn in *. 
+    specialize (HEnc Fin0) as HEnc0; specialize (HEnc Fin1) as HEnc1. cbn in *. 
+    cbn in *; simpl_vector in *; cbn in *.
+    modpon H. intros i; destruct_fin i; cbn in *; eauto.
+  - intros tin k HEnc. cbn in *.
+    specialize (HEnc Fin0) as HEnc0; specialize (HEnc Fin1) as HEnc1.
+    cbn in *; simpl_vector in *; cbn in *. eauto.
+Qed.
+
+(** Recover version without space is easy. Normally, we wouldn't write down this lemma because the automation takes care of everything. (But not for [CopyValue], etc!) *)
+Lemma CopyValue_SpecT (sig : finType) (sigX X : Type) (cX : codable sigX X) (I : Retract sigX sig) (x : X) :
+  TripleT (tspec (SpecVector [|Contains _ x; Void|])) (CopyValue_steps x) (CopyValue _) (fun _ => tspec (SpecVector [|Contains _ x; Contains _ x|])).
+Proof. eapply TripleT_RemoveSpace. cbn. intros s. apply CopyValue_SpecT_size. Qed.
+
+
+Lemma Reset_SpecT_space (sig : finType) (sigX X : Type) (cX : codable sigX X) (I : Retract sigX sig) (x : X) (ss : Vector.t nat 1) :
+  TripleT (tspec (withSpace (SpecVector [|Contains _ x|]) ss)) (Reset_steps x) (Reset _) (fun _ => tspec (withSpace (SpecVector [|Void|]) (appSize [|Reset_size x|] ss))).
+Proof.
+  eapply Realise_TripleT.
+  - apply Reset_Realise.
+  - apply Reset_Terminates.
+  - intros tin [] tout H HEnc. cbn in *.
+    specialize (HEnc Fin0); cbn in *. simpl_vector in *; cbn in *.
+    modpon H. intros i; destruct_fin i; cbn; eauto.
+  - intros tin k HEnc. cbn in *.
+    specialize (HEnc Fin0). simpl_vector in *; cbn in *. eauto.
+Qed.
+
+(** This would also not normally be written down. *)
+Lemma Reset_SpecT (sig : finType) (sigX X : Type) (cX : codable sigX X) (I : Retract sigX sig) (x : X) :
+  TripleT (tspec (SpecVector [|Contains _ x|])) (Reset_steps x) (Reset _) (fun _ => tspec (SpecVector [|Void|])).
+Proof. eapply TripleT_RemoveSpace. apply Reset_SpecT_space. Qed.
+
+(** This would also not normally be written down. *)
+Lemma Reset_Spec (sig : finType) (sigX X : Type) (cX : codable sigX X) (I : Retract sigX sig) (x : X) :
+  Triple (tspec (SpecVector [|Contains _ x|])) (Reset _) (fun _ => tspec (SpecVector [|Void|])).
+Proof. eapply TripleT_Triple. apply Reset_SpecT. Qed.
+
+
+(** Important: The types ([X] and [Y]) or the retractions ([I1] and [I2]) have to be manually instantiated when using these lemmas. *)
+(** (With some "non-standard" encodings, the encodings have to be instantiated, of course.) *)
+
+(* TODO: Move to [Code/Copy.v] *)
+Definition MoveValue_size {X Y sigX sigY : Type} {cX : codable sigX X} {cY : codable sigY Y} (x : X) (y : Y) : Vector.t (nat->nat) 2 :=
+  [|MoveValue_size_x x; MoveValue_size_y x y|].
+
+Lemma MoveValue_SpecT_size (sig : finType) (sigX sigY X Y : Type)
+      (cX : codable sigX X) (cY : codable sigY Y) (I1 : Retract sigX sig) (I2 : Retract sigY sig) (x : X) (y : Y) (ss : Vector.t nat 2) :
+  TripleT (tspec (withSpace (SpecVector [|Contains _ x; Contains _ y|]) ss)) (MoveValue_steps x y) (MoveValue _)
+          (fun _ => tspec (withSpace (SpecVector [|Void; Contains _ x|]) (appSize (MoveValue_size x y) ss))).
+Proof.
+  eapply Realise_TripleT.
+  - apply MoveValue_Realise with (X := X) (Y := Y).
+  - apply MoveValue_Terminates with (X := X) (Y := Y).
+  - intros tin [] tout H HEnc. cbn in *.
+    specialize (HEnc Fin0) as HEnc0; specialize (HEnc Fin1) as HEnc1. simpl_vector in *; cbn in *.
+    modpon H. intros i; destruct_fin i; cbn; eauto.
+  - intros tin k HEnc. cbn in *.
+    specialize (HEnc Fin0) as HEnc0; specialize (HEnc Fin1) as HEnc1. simpl_vector in *; cbn in *. eauto.
+Qed.
+
+Lemma MoveValue_SpecT (sig : finType) (sigX sigY X Y : Type)
+      (cX : codable sigX X) (cY : codable sigY Y) (I1 : Retract sigX sig) (I2 : Retract sigY sig) (x : X) (y : Y) :
+  TripleT (tspec (SpecVector [|Contains _ x; Contains _ y|])) (MoveValue_steps x y) (MoveValue _) (fun _ => tspec (SpecVector [|Void; Contains _ x|])).
+Proof. eapply TripleT_RemoveSpace. apply MoveValue_SpecT_size. Qed.
+
+Lemma MoveValue_Spec (sig : finType) (sigX sigY X Y : Type)
+      (cX : codable sigX X) (cY : codable sigY Y) (I1 : Retract sigX sig) (I2 : Retract sigY sig) (x : X) (y : Y) :
+  Triple (tspec (SpecVector [|Contains _ x; Contains _ y|])) (MoveValue _) (fun _ => tspec (SpecVector [|Void; Contains _ x|])).
+Proof. eapply TripleT_Triple. apply MoveValue_SpecT. Qed.
+
+
+(** For the abve reasons, we must not add these tactics to the automation! (As in [TM_Correct].) *)
+
+(** *** Constructors for [nat] *)
+
+(** Pure triple (without register specification language); only for demonstration *)
+Lemma Constr_O_SpecT_pure :
+  TripleT (fun tin => isVoid tin[@Fin0]) (Constr_O_steps) (Constr_O) (fun _ tout => tout[@Fin0] ≃ 0).
+Proof.
+  eapply RealiseIn_TripleT.
+  - apply Constr_O_Sem.
+  - intros tin [] tout H1 H2. cbn in *. unfold tspec in *. modpon H1. contains_ext.
+Qed.
+
+Lemma Constr_O_Spec_pure :
+  Triple (fun tin => isVoid tin[@Fin0]) (Constr_O) (fun _ tout => tout[@Fin0] ≃ 0).
+Proof. eapply TripleT_Triple. apply Constr_O_SpecT_pure. Qed.
+
+Lemma Constr_S_SpecT_pure (y : nat) :
+  TripleT (fun tin => tin[@Fin0] ≃ y) (Constr_S_steps) (Constr_S) (fun _ tout => tout[@Fin0] ≃ S y).
+Proof.
+  eapply RealiseIn_TripleT.
+  - apply Constr_S_Sem.
+  - intros tin [] tout H1 H2. cbn in *. unfold tspec in *. modpon H1. contains_ext.
+Qed.
+
+Lemma Constr_S_Spec_pure (y : nat) :
+  Triple (fun tin => tin[@Fin0] ≃ y) (Constr_S) (fun _ tout => tout[@Fin0] ≃ (S y)).
+Proof. eapply TripleT_Triple. apply Constr_S_SpecT_pure. Qed.
+
+
+(** Expressed using the specification language *)
+
+Lemma Constr_O_SpecT_size (ss : Vector.t nat 1) :
+  TripleT (tspec (withSpace (SpecVector [|Void|]) ss)) Constr_O_steps Constr_O (fun _ => tspec (withSpace (SpecVector [|Contains _ 0|]) (appSize [|Constr_O_size|] ss))).
+Proof.
+  eapply RealiseIn_TripleT.
+  - apply Constr_O_Sem.
+  - intros tin [] tout H1 H2. cbn in *. unfold tspec in *. specialize (H2 Fin0). simpl_vector in *; cbn in *. modpon H1.
+    hnf. intros i; destruct_fin i; cbn; eauto.
+Qed.
+
+Lemma Constr_O_SpecT :
+  TripleT (tspec (SpecVector [|Void|])) Constr_O_steps Constr_O (fun _ => tspec (SpecVector [|Contains _ 0|])).
+Proof. eapply TripleT_RemoveSpace; apply Constr_O_SpecT_size. Qed.
+
+Lemma Constr_O_Spec :
+  Triple (tspec (SpecVector [|Void|])) Constr_O (fun _ => tspec (SpecVector [|Contains _ 0|])).
+Proof. eapply TripleT_Triple. apply Constr_O_SpecT. Qed.
+
+Lemma Constr_S_SpecT_size :
+  forall (y : nat) ss,
+    TripleT (tspec (withSpace (SpecVector [|Contains _ y|]) ss)) Constr_S_steps Constr_S
+            (fun _ => tspec (withSpace (SpecVector [|Contains _ (S y)|]) (appSize [|S|] ss))).
+Proof.
+  intros y ss.
+  eapply RealiseIn_TripleT.
+  - apply Constr_S_Sem.
+  - intros tin [] tout H HEnc. cbn in *.
+    specialize (HEnc Fin0). simpl_vector in *; cbn in *. modpon H.
+    hnf. intros i; destruct_fin i; cbn; eauto.
+Qed.
+
+Lemma Constr_S_SpecT :
+  forall (y : nat), TripleT (tspec (SpecVector [|Contains _ y|])) Constr_S_steps Constr_S (fun _ => tspec (SpecVector [|Contains _ (S y)|])).
+Proof. intros. eapply TripleT_RemoveSpace; apply Constr_S_SpecT_size. Qed.
+
+Lemma Constr_S_Spec :
+  forall (y : nat), Triple (tspec (SpecVector [|Contains _ y|])) Constr_S (fun _ => tspec (SpecVector [|Contains _ (S y)|])).
+Proof. intros y. eapply TripleT_Triple. apply Constr_S_SpecT. Qed.
+
+
+(** For the deconstructor, we have the same weird [match] as in the Realisation rules. Note, that [tspec] must be the head of the expression.
+This is way we had to embed [SpecFalse] as a [Spec]. *)
+
+Definition CaseNat_size (n : nat) : Vector.t (nat->nat) 1 :=
+  match n with
+  | O => [|id|]
+  | S n' => [|S|]
+  end.
+
+Lemma CaseNat_SpecT_size (y : nat) (ss : Vector.t nat 1) :
+  TripleT
+    (tspec (withSpace (SpecVector [|Contains _ y|]) ss))
+    CaseNat_steps
+    CaseNat
+    (fun yout =>
+       tspec
+         (withSpace
+            (match yout, y with
+             | true, S y' => SpecVector [|Contains _ y'|]
+             | false, 0 => SpecVector [|Contains _ 0|]
+             | _, _ => SpecFalse
+             end)
+            (appSize (CaseNat_size y) ss))). (** Note that we add [withSpac] between the [tspec] and the [match] *)
+Proof.
+  eapply RealiseIn_TripleT.
+  - apply CaseNat_Sem.
+  - intros tin yout tout H HEnc. specialize (HEnc Fin0). simpl_vector in *; cbn in *. modpon H.
+    destruct yout, y; cbn in *; auto.
+    + hnf. intros i; destruct_fin i; cbn; eauto.
+    + hnf. intros i; destruct_fin i; cbn; eauto.
+Qed.
+
+Lemma CaseNat_SpecT (y : nat) :
+  TripleT
+    (tspec (SpecVector [|Contains _ y|]))
+    CaseNat_steps
+    CaseNat
+    (fun yout =>
+       tspec
+         match yout, y with
+         | true, S y' => SpecVector [|Contains _ y'|]
+         | false, 0 => SpecVector [|Contains _ 0|]
+         | _, _ => SpecFalse
+         end).
+Proof. eapply TripleT_RemoveSpace. apply CaseNat_SpecT_size. Qed.
+
+Lemma CaseNat_Spec (y : nat) :
+  Triple (tspec (SpecVector [|Contains _ y|]))
+         CaseNat
+         (fun yout =>
+            tspec
+              match yout, y with
+              | true, S y' => SpecVector [|Contains _ y'|]
+              | false, 0 => SpecVector [|Contains _ 0|]
+              | _, _ => SpecFalse
+              end).
+Proof. eapply TripleT_Triple. apply CaseNat_SpecT. Qed.
+
+
+(** A combination of the consequence rule and the above correctness lemma. (The automation also takes care of this.) *)
+Lemma Constr_S_Spec_con (n : nat) (Q : Assert sigNat^+ 1) :
+  (forall tout, tspec (SpecVector [|Contains _ (S n)|]) tout -> Q tout) ->
+  Triple (tspec (SpecVector [|Contains _ n|])) Constr_S (fun _ => Q).
+Proof. eauto using Consequence_post, Constr_S_Spec. Qed.
+
+
+
+(** Add all [nat] (de)constructor lemmas to the automation. We only have to register the complete correctness lemmas. *)
+(** Here we demonstrate how to register specifications to the automation. We only have to register the strongest proven variant, e.g. with time & space.
+All other (weaker) variants will be derived by the automation on-the-fly, if needed. *)
+Ltac hstep_Nat :=
+  lazymatch goal with
+  | [ |- TripleT ?P ?k Constr_O ?Q ] => eapply Constr_O_SpecT_size
+  (* We only use register-machines. There is no need to have lemmas without register specifications. This was only done here for demonstration purposes. *)
+  | [ |- TripleT ?P ?k Constr_S ?Q ] => eapply Constr_S_SpecT_size
+  | [ |- TripleT ?P ?k CaseNat ?Q ] => eapply CaseNat_SpecT_size
+  end.
+
+Smpl Add hstep_Nat : hstep_smpl.
+
+
+
+(** *** A simple example *)
+
+(** Pure example: increment a number twice *)
+
+Definition IncrementTwice_steps := 1 + Constr_S_steps + Constr_S_steps.
+
+Definition IncrementTwice : pTM sigNat^+ unit 1 := Constr_S;; Constr_S.
+
+Lemma IncrementTwice_Spec_pure (y : nat) :
+  Triple (fun tin => tin[@Fin0] ≃ y) (IncrementTwice) (fun _ tout => tout[@Fin0] ≃ S (S y)).
+Proof.
+  eapply Seq_Spec.
+  - apply Constr_S_Spec_pure.
+  - cbn. intros _. apply Constr_S_Spec_pure.
+Restart.
+  unfold IncrementTwice. (* Because the automation is working syntactically, the definition has first to be unfolded (like in [TM_Correct]). *)
+  hsteps. apply Constr_S_Spec_pure.
+  cbn. intros _. apply Constr_S_Spec_pure.
+Qed.
+
+(** With time! *)
+Lemma IncrementTwice_SpecT_pure (y : nat) :
+  TripleT (fun tin => tin[@Fin0] ≃ y) (IncrementTwice_steps) (IncrementTwice) (fun _ tout => tout[@Fin0] ≃ S (S y)).
+Proof.
+  eapply Seq_SpecT.
+  - apply Constr_S_SpecT_pure.
+  - cbn. intros _. apply Constr_S_SpecT_pure.
+  - reflexivity. (* Easy! *)
+Restart.
+  unfold IncrementTwice. hsteps. apply Constr_S_SpecT_pure.
+  cbn. intros _. apply Constr_S_SpecT_pure.
+  reflexivity.
+Qed.
+
+
+
+(** Same example, but using the specification language *)
+
+Lemma IncrementTwice_Spec (y : nat) :
+  Triple (tspec (SpecVector [|Contains _ y|])) (IncrementTwice) (fun _ => tspec (SpecVector [|Contains _ (S (S y))|])).
+Proof.
+  eapply Seq_Spec.
+  - apply Constr_S_Spec.
+  - cbn. intros _. apply Constr_S_Spec.
+Restart. (* Proof with step-by-step automation and without the user-defined tactic for [Constr_S]. *)
+  unfold IncrementTwice. hstep. apply Constr_S_Spec.
+  cbn. intros _.
+  apply Constr_S_Spec. (* We can directly use [Constr_S_Spec] here, because the postconditions match syntactically. This usually not the case. *)
+Restart.
+  unfold IncrementTwice.
+  hsteps_cbn. eauto.
+  (* The automation always applies the Consequence rule for user-defined specifications, if the postcondition is not an evar. *)
+  (* The version [hstep_cbn] calls [cbn] before each step. [forall (x : unit)] will be automatically removed. *)
+  (* Note that [hstep_user] automatically converted [Constr_S_SpecT_size] to [Constr_S_Spec]. It can handle all combinations of such weakenings. *)
+Qed.
+
+Lemma IncrementTwice_SpecT (y : nat) :
+  TripleT (tspec (SpecVector [|Contains _ y|])) (IncrementTwice_steps) (IncrementTwice) (fun _ => tspec (SpecVector [|Contains _ (S (S y))|])).
+Proof.
+  eapply Seq_SpecT.
+  - apply Constr_S_SpecT.
+  - cbn. intros _. apply Constr_S_SpecT.
+  - reflexivity.
+Restart.
+  unfold IncrementTwice. hstep. apply Constr_S_SpecT.
+  cbn. intros _. apply Constr_S_SpecT. (* We can directly use [Constr_S_Spec'] here, because the postconditions match syntactically. This usually not the case. *)
+Restart. (* Full automation! *)
+  unfold IncrementTwice. hsteps_cbn.
+  eauto. reflexivity. (* This is easy, isn't it? *)
+Qed.
+
+
+
+(** Example using the specification language and lifting: Increment two numbers *)
+
+Definition Incr2 : pTM sigNat^+ unit 2 :=
+  Constr_S@[|Fin0|];; Constr_S@[|Fin1|].
+
+Definition Incr2_steps := 1 + Constr_S_steps + Constr_S_steps.
+
+
+
+Lemma Incr2_Spec :
+  forall (x y : nat), Triple (tspec (SpecVector [|Contains _ x; Contains _ y|])) Incr2 (fun _ => tspec (SpecVector [|Contains _ (S x); Contains _ (S y)|])).
+Proof.
+  intros x y.
+  eapply Seq_Spec.
+  - eapply LiftTapes_Spec.
+    + smpl_dupfree.
+    + cbn. apply Constr_S_Spec.
+  - cbn. intros _. eapply LiftTapes_Spec_con. (* For the last step, we have to use the lifting rule with consequence rule. *)
+    + smpl_dupfree.
+    + cbn. apply Constr_S_Spec.
+    + cbn. auto.
+      (* After the last step, we have to prove that our "generated" assertion implies the wanted assertion. *)
+      (* The prove is completed with simplification. The HUGE advantage is that we never have to rewrite anything! *)
+      (* The proof is faster than using realisation directly. *)
+Restart.
+  (* The tactics can do this automatically *)
+  intros x y. unfold Incr2.
+  hsteps_cbn. eauto.
+Qed.
+
+Lemma Incr2_SpecT :
+  forall (x y : nat), TripleT (tspec (SpecVector [|Contains _ x; Contains _ y|])) Incr2_steps Incr2 (fun _ => tspec (SpecVector [|Contains _ (S x); Contains _ (S y)|])).
+Proof.
+  intros x y.
+  eapply Seq_SpecT.
+  - eapply LiftTapes_SpecT.
+    + smpl_dupfree.
+    + cbn. apply Constr_S_SpecT.
+  - intros []. cbn [Frame]. eapply LiftTapes_SpecT_con.
+    + smpl_dupfree.
+    + cbn. apply Constr_S_SpecT.
+    + cbn. auto.
+  - reflexivity.  (* <- This is the only difference to the above lemma (without time)! We actually don't need to prove [Incr2_Spec] first. *)
+Restart.
+  intros x y. unfold Incr2. hsteps_cbn. eauto. reflexivity.
+Qed.
+
+
+
+
+(** More increments *)
+
+Definition Incr3 : pTM sigNat^+ unit 3 :=
+  Constr_S@[|Fin0|];; Constr_S@[|Fin1|];; IncrementTwice@[|Fin2|].
+
+Definition Incr3_steps := 2 + Constr_S_steps + Constr_S_steps + IncrementTwice_steps.
+
+Lemma Incr3_Spec :
+  forall (x y z : nat), Triple (tspec (SpecVector [|Contains _ x; Contains _ y; Contains _ z|])) Incr3 (fun _ => tspec (SpecVector [|Contains _ (S x); Contains _ (S y); Contains _ (S (S z))|])).
+Proof.
+  intros x y z.
+  eapply Seq_Spec.
+  - eapply LiftTapes_Spec.
+    + smpl_dupfree.
+    + cbn. apply Constr_S_Spec.
+  - intros []. cbn [Frame].
+    eapply Seq_Spec. (* The second Seq just works as the first one. *)
+    + eapply LiftTapes_Spec.
+      * smpl_dupfree.
+      * cbn. apply Constr_S_Spec.
+    + intros []. cbn [Frame].
+      eapply LiftTapes_Spec_con. (* We again have to use the lifting rule with the consequence rule here. *)
+      * smpl_dupfree.
+      * cbn. apply IncrementTwice_Spec.
+      * cbn. auto. (* Done! *)
+Restart.
+  intros x y z. unfold Incr3.
+  hsteps_cbn. apply IncrementTwice_Spec. cbn. eauto.
+Qed.
+
+(** The same with time! *)
+Lemma Incr3_SpecT :
+  forall (x y z : nat), TripleT (tspec (SpecVector [|Contains _ x; Contains _ y; Contains _ z|])) (Incr3_steps) Incr3 (fun _ => tspec (SpecVector [|Contains _ (S x); Contains _ (S y); Contains _ (S (S z))|])).
+Proof.
+  intros x y z.
+  eapply Seq_SpecT.
+  - eapply LiftTapes_SpecT.
+    + smpl_dupfree.
+    + cbn. apply Constr_S_SpecT.
+  - intros []. cbn [Frame].
+    eapply Seq_SpecT.
+    + eapply LiftTapes_SpecT.
+      * smpl_dupfree.
+      * cbn. apply Constr_S_SpecT.
+    + intros []. cbn [Frame].
+      eapply LiftTapes_SpecT_con.
+      * smpl_dupfree.
+      * cbn. apply IncrementTwice_SpecT.
+      * cbn. auto.
+    + reflexivity. (* first difference *)
+  - reflexivity. (* second difference *)
+Restart.
+  intros x y z. unfold Incr3.
+  hsteps_cbn. apply IncrementTwice_SpecT. cbn. eauto. reflexivity. reflexivity.
+Qed.
+
+
+
+(** *** Addition *)
+
+
+Definition Add_Step : pTM sigNat^+ (option unit) 2 :=
+  If (CaseNat @ [|Fin1|])
+     (Return (Constr_S @ [|Fin0|]) None)
+     (Return Nop (Some tt)).
+
+(*
+Definition Add_Step_Rel : pRel sigNat^+ (option unit) 2 :=
+  fun tin '(yout, tout) =>
+    forall a b sa sb,
+      tin [@Fin0] ≃(;sa) a ->
+      tin [@Fin1] ≃(;sb) b ->
+      match yout, b with
+      | Some tt, O => (* break *)
+        tout[@Fin0] ≃(;sa) a /\
+        tout[@Fin1] ≃(;sb) b
+      | None, S b' =>
+        tout[@Fin0] ≃(;pred sa) S a /\
+        tout[@Fin1] ≃(;S sb) b'
+      | _, _ => False
+      end.
+*)
+
+
+Definition Add_Step_Post : nat*nat -> option unit -> Assert sigNat^+ 2 :=
+  fun '(a,b) =>
+  (fun yout =>
+     tspec
+       match yout, b with
+       | Some _, 0 => SpecVector [|Contains _ a; Contains _ b|]
+       | None, S b' => SpecVector [|Contains _ (S a); Contains _ b'|]
+       | _, _ => SpecFalse
+       end).
+
+Lemma Add_Step_Spec (a b : nat) :
+  Triple (tspec (SpecVector [|Contains _ a; Contains _ b|])) Add_Step
+         (Add_Step_Post (a,b)).
+Proof.
+  eapply If_Spec.
+  - apply LiftTapes_Spec.
+    + smpl_dupfree.
+    + cbn. eapply CaseNat_Spec.
+  - cbn. destruct b as [ | b']; cbn [Frame]; eauto.
+    eapply Return_Spec_con.
+    + cbn [Vector.nth Vector.caseS Vector.case0].
+      apply LiftTapes_Spec.
+      * smpl_dupfree.
+      * cbn [Downlift select]. apply Constr_S_Spec.
+    + intros []. auto.
+  - cbn. destruct b as [ | b']; cbn [Frame]; eauto.
+    eapply Return_Spec_con.
+    + cbn [Vector.nth Vector.caseS Vector.case0]. apply Nop_Spec.
+    + intros []. auto.
+Qed.
+
+Definition Add_Loop : pTM sigNat^+ unit 2 := While Add_Step.
+
+(*
+Definition Add_Loop_Rel : pRel sigNat^+ unit 2 :=
+  ignoreParam (
+      fun tin tout =>
+        forall a b sa sb,
+          tin [@Fin0] ≃(;sa) a ->
+          tin [@Fin1] ≃(;sb) b ->
+          tout[@Fin0] ≃(;sa-b) b + a /\
+          tout[@Fin1] ≃(;sb+b) 0
+    ).
+*)
+
+Lemma Add_Loop_Spec (a b : nat) :
+  Triple (tspec (SpecVector [|Contains _ a; Contains _ b|]))
+         Add_Loop
+         (fun _ => tspec (SpecVector [|Contains _ (a+b); Contains _ 0|])).
+Proof.
+  eapply While_Spec with
+      (P := fun '(a,b) => _)
+      (* (Q := _) (* to be instantiated by the first proof obligation *) *)
+      (R := fun '(a,b) => _) (x := (a,b)).
+  - intros (x,y). apply Add_Step_Spec. (* Instantiate correctness of [AddStep] *)
+  - intros (x,y) yout tmid tout H. cbn in *. (* Termination case *)
+    destruct y as [ | y']; cbn in *; auto.
+    intros H1 H3. replace (x+0) with x by omega. auto.
+  - intros (x,y) tin tmid H1 H2. cbn in *.
+    destruct y as [ | y']; cbn in *; auto.
+    eexists (_,_); cbn. split.
+    + eauto.
+    + intros _ tout. replace (S x + y') with (x + S y') by omega. auto.
+Qed.
+
+
+
+(** The same with termination! *)
+
+Definition Add_Step_steps : nat := 9.
+
+Lemma Add_Step_SpecT (a b : nat) :
+  TripleT (tspec (SpecVector [|Contains _ a; Contains _ b|]))
+          Add_Step_steps
+          Add_Step
+         (Add_Step_Post (a,b)).
+Proof.
+  eapply If_SpecT_weak'.
+  - apply LiftTapes_SpecT.
+    + smpl_dupfree.
+    + cbn. eapply CaseNat_SpecT.
+  - cbn. destruct b as [ | b']; cbn [Frame]; eauto.
+    eapply Return_SpecT_con.
+    + cbn [Vector.nth Vector.caseS Vector.case0].
+      apply LiftTapes_SpecT.
+      * smpl_dupfree.
+      * cbn [Downlift select]. apply Constr_S_SpecT.
+    + intros []. auto.
+  - cbn. destruct b as [ | b']; cbn [Frame]; eauto.
+    eapply Return_SpecT_con.
+    + cbn. apply Nop_SpecT_con.
+    + intros []. auto.
+  - reflexivity.
+Restart.
+  unfold Add_Step.
+  eapply If_SpecT_weak'.
+  - hsteps.
+  - destruct b as [ | b']; cbn in *; auto.
+    hsteps. cbn. eauto.
+  - destruct b as [ | b']; cbn in *; auto.
+    hsteps. cbn.
+    apply Nop_SpecT_con. cbn. eauto. (* We have to manually use other rule for [Nop] here. *)
+  - reflexivity.
+Restart. (* With [If_SpecT] *)
+  (* It is important to do the [destruct] before other steps. So we are a bit carefull here. *)
+  (* We also have to instantiate the step number for [M3] to [0] manually, because of a Coq bug. We don't have to do it if it isn't [0]. *)
+  unfold Add_Step. eapply If_SpecT with (k3 := 0).
+  - hsteps.
+  - destruct b as [ | b']; cbn in *; auto.
+    hsteps. cbn. eauto.
+  - destruct b as [ | b']; cbn in *; auto.
+    hsteps. cbn. eauto.
+  - intros. destruct yout. reflexivity. unfold CaseNat_steps, Add_Step_steps. omega.
+Qed.
+
+
+
+(** With space *)
+
+
+
+Definition Add_Step_size (a b : nat) : Vector.t (nat->nat) 2 :=
+  match b with
+  | 0 => [|id; id|]
+  | S b' => [|S; S|]
+  end.
+
+Lemma Add_Step_SpecT_space (a b : nat) (ss : Vector.t nat 2) :
+  TripleT
+    (tspec (withSpace (SpecVector [|Contains _ a; Contains _ b|]) ss))
+    Add_Step_steps
+    Add_Step
+    (fun yout =>
+       tspec
+         (withSpace match yout, b with
+                    | Some _, 0 => SpecVector [|Contains _ a; Contains _ b|]
+                    | None, S b' => SpecVector [|Contains _ (S a); Contains _ b'|]
+                    | _, _ => SpecFalse
+                    end
+         (appSize (Add_Step_size a b) ss))).
+Proof.
+  unfold Add_Step. eapply If_SpecT with (k3 := 0).
+  - hsteps_cbn.
+  - destruct b as [ | b']; cbn in *; auto. hsteps_cbn; cbn. auto.
+  - destruct b as [ | b']; cbn in *; auto.
+    hsteps. cbn. cbn. eauto.
+  - intros. destruct yout. (* reflexivity. unfold CaseNat_steps, Add_Step_steps. omega. *)
+    + reflexivity.
+    + unfold CaseNat_steps, Add_Step_steps. omega.
+Qed.
+
+
+
+Definition Add_Loop_steps b := 9 + 10 * b.
+
+
+Lemma Add_Loop_SpecT (a b : nat) :
+  TripleT (tspec (SpecVector [|Contains _ a; Contains _ b|]))
+          (Add_Loop_steps b)
+          (Add_Loop)
+          (fun _ => tspec (SpecVector [|Contains _ (a+b); Contains _ 0|])).
+Proof.
+  (* Unification can instantiate the abstractions for us. *)
+  eapply While_SpecT with (P := fun '(a,b) => _) (R := fun '(a,b) => _) (f := fun '(a,b) => _) (g := fun '(a,b) => _) (x := (a,b)).
+    - intros (x,y). apply Add_Step_SpecT. (* Instantiate correctness of [AddStep] *)
+    - intros (x,y) yout tout Post. cbn in *.
+      destruct y as [ | y']; cbn in *; auto.
+      intros H1 H2. replace (x+0) with x by omega. auto.
+    - intros (x,y); intros.
+      destruct y as [ | y']; cbn in *; auto.
+      eexists (S x, y') (* or [eexists (_,_)] *); cbn. repeat split.
+      + eauto.
+      + unfold Add_Step_steps, Add_Loop_steps. omega.
+      + replace (S x + y') with (x + S y') by omega. auto.
+Qed.
+
+Fixpoint Add_Loop_size (a b : nat) : Vector.t (nat->nat) 2 :=
+  match b with
+  | O => Add_Step_size a b
+  | S b' => Add_Step_size a b >>> Add_Loop_size (S a) b'
+  end.
+
+Opaque Triple TripleT.
+
+Lemma Add_Loop_SpecT_size (a b : nat) (ss : Vector.t nat 2) :
+  TripleT
+    (tspec (withSpace (SpecVector [|Contains _ a; Contains _ b|]) ss))
+    (Add_Loop_steps b)
+    (Add_Loop)
+    (fun _ => tspec
+             (withSpace
+                (SpecVector [|Contains _ (a+b); Contains _ 0|])
+                (appSize (Add_Loop_size a b) ss))).
+Proof.
+  (** We have to add the space vector to the abstract state *)
+  eapply While_SpecT with (P := fun '(a,b,ss) => _) (Q := fun '(a,b,ss) => _) (R := fun '(a,b,ss) => _) (f := fun '(a,b,ss) => _) (g := fun '(a,b,ss) => _) (x := (a,b,ss));
+    clear a b ss; intros ((x,y),ss).
+    - apply Add_Step_SpecT_space.
+    - intros [] tmid tout H1 H2.
+      destruct y as [ | y']; cbn in *; auto.
+      replace (x+0) with x by omega. split; eauto.
+    - intros tin tmid H1 H2.
+      destruct y as [ | y']; cbn in *; auto.
+      eexists (S x, y', _); cbn. repeat split.
+      + eauto.
+      + unfold Add_Step_steps, Add_Loop_steps. omega.
+      + replace (S x + y') with (x + S y') by omega. auto.
+Qed.
+
+
+Definition Add : pTM sigNat^+ unit 4 :=
+  LiftTapes (CopyValue _) [|Fin1; Fin2|];; (* copy n to a *)
+  LiftTapes (CopyValue _) [|Fin0; Fin3|];; (* copy m to b *)
+  LiftTapes Add_Loop [|Fin2; Fin3|];; (* Main loop *)
+  LiftTapes (Reset _) [|Fin3|]. (* Reset b *)
+
+Definition Add_steps m n := 98 + 12 * n + 22 * m.
+
+Lemma Add_SpecT (a b : nat) :
+  TripleT (tspec (SpecVector [|Contains _ a; Contains _ b; Void; Void|]))
+          (Add_steps a b)
+          Add
+          (fun _ => tspec (SpecVector [|Contains _ a; Contains _ b; Contains _ (a+b); Void|])).
+Proof.
+  eapply Seq_SpecT.
+  eapply LiftTapes_SpecT. smpl_dupfree. eapply CopyValue_SpecT.
+  intros []. cbn.
+  eapply Seq_SpecT.
+  eapply LiftTapes_SpecT. smpl_dupfree. eapply CopyValue_SpecT.
+  intros []. cbn.
+  eapply Seq_SpecT.
+  apply LiftTapes_SpecT. smpl_dupfree. cbn. apply Add_Loop_SpecT.
+  cbn. intros _.
+  eapply LiftTapes_SpecT_con. smpl_dupfree. eapply Reset_SpecT.
+  cbn. intros _ tout. replace (a+b) with (b+a) by omega. auto.
+  reflexivity. reflexivity.
+  unfold CopyValue_steps, Add_Loop_steps, Add_steps, Reset_steps. rewrite !Encode_nat_hasSize. omega.
+Restart.
+  unfold Add. hsteps_cbn. eapply CopyValue_SpecT. apply CopyValue_SpecT. apply Add_Loop_SpecT. cbn. apply Reset_SpecT. cbn.
+  (* The only interesting part of the proof! *)
+  replace (a+b) with (b+a) by omega. auto.
+  reflexivity. reflexivity.
+  unfold CopyValue_steps, Add_Loop_steps, Add_steps, Reset_steps. rewrite !Encode_nat_hasSize. omega.
+Qed.
+
+
+Definition Add_space (a b : nat) : Vector.t (nat->nat) 4 :=
+  [|(*0*) id; (*1*) id; (*2*) CopyValue_size b >> Add_Loop_size b a @>Fin0;
+      (*3*) CopyValue_size a >> (Add_Loop_size b a @>Fin1) >> Reset_size 0 |].
+
+(*
+(* Optional *)
+Arguments appSize : simpl never.
+*)
+
+Lemma Add_SpecT_space (a b : nat) (ss : Vector.t nat 4) :
+  TripleT
+    (tspec (withSpace (SpecVector [|Contains _ a; Contains _ b; Void; Void|]) ss))
+    (Add_steps a b)
+    Add
+    (fun _ => tspec (withSpace (SpecVector [|Contains _ a; Contains _ b; Contains _ (a+b); Void|])
+                            (appSize (Add_space a b) ss))).
+Proof. (* The tactic [hstep] takes also takes care of moving [withSpace] to the head symbol of each precondition *)
+  unfold Add.
+  hstep. hstep.
+  apply CopyValue_SpecT_size.
+  cbn. intros _. cbn.
+  hstep. cbn. hstep. cbn. apply CopyValue_SpecT_size.
+  cbn. intros _. hstep. cbn. hstep. cbn. apply Add_Loop_SpecT_size.
+  cbn. intros _. hstep. cbn. apply Reset_SpecT_space.
+  cbn. intros _. replace (b+a) with (a+b) by omega. auto.
+  reflexivity. reflexivity.
+  unfold CopyValue_steps, Reset_steps, Add_Loop_steps, Add_steps. rewrite !Encode_nat_hasSize. omega.
+Qed.
+
+
+(** *** Multiplication *)
+
+Definition Mult_Step : pTM sigNat^+ (option unit) 5 :=
+  If (LiftTapes CaseNat [|Fin0|])
+     (Return (
+          LiftTapes Add [|Fin1; Fin2; Fin3; Fin4|];; (* Add(n, c, c') *)
+          LiftTapes (MoveValue _) [|Fin3; Fin2|]
+        ) (None)) (* continue *)
+     (Return Nop (Some tt)). (* break *)
+
+
+(* (* For comparison: The correctness relation of [Mult_Step] (with space) *)
+Definition Mult_Step_Rel : pRel sigNat^+ (option unit) 5 :=
+  fun tin '(yout, tout) =>
+    forall (c m' n : nat) (sm sn sc s3 s4 : nat),
+      tin[@Fin0] ≃(;sm) m' ->
+      tin[@Fin1] ≃(;sn) n ->
+      tin[@Fin2] ≃(;sc) c ->
+      isVoid_size tin[@Fin3] s3 ->
+      isVoid_size tin[@Fin4] s4 ->
+      match yout, m' with
+      | (Some tt), O => (* return *)
+        tout[@Fin0] ≃(;sm) m' /\
+        tout[@Fin1] ≃(;sn) n /\
+        tout[@Fin2] ≃(;sc) c /\
+        isVoid_size tout[@Fin3] s3 /\
+        isVoid_size tout[@Fin4] s4
+      | None, S m'' => (* continue *)
+        tout[@Fin0] ≃(;S sm) m'' /\
+        tout[@Fin1] ≃(;sn) n /\
+        tout[@Fin2] ≃(;sc-n) n + c /\
+        isVoid_size tout[@Fin3] (2 + n + c + Add_space2 n c s3)  /\
+        isVoid_size tout[@Fin4] (Add_space3 n s4)
+      | _, _ => False
+      end.
+*)
+
+Definition Mult_Step_Post : nat*nat*nat -> option unit -> Assert sigNat^+ 5 :=
+  fun '(m',n,c) =>
+  (fun yout =>
+     tspec
+       match yout, m' with
+       | Some _, 0 => SpecVector [|Contains _ m'; Contains _ n; Contains _ c; Void; Void|]
+       | None, S m'' => SpecVector [|Contains _ m''; Contains _ n; Contains _ (n+c); Void; Void|]
+       | _, _ => SpecFalse
+       end).
+
+Definition Mult_Step_steps m' n c :=
+  match m' with
+  | O => 6
+  | _ => 168 + 33 * c + 39 * n
+  end.
+
+
+(** We need the strong version [If_SpecT_strong] here, becaue the running time depends on the path *)
+Lemma Mult_Step_SpecT m' n c :
+  TripleT
+    (tspec (SpecVector [|Contains _ m'; Contains _ n; Contains _ c; Void; Void|]))
+    (Mult_Step_steps m' n c)
+    (Mult_Step)
+    ((Mult_Step_Post) (m',n,c)).
+Proof.
+  eapply If_SpecT.
+  - apply LiftTapes_SpecT. smpl_dupfree. cbn. apply CaseNat_SpecT.
+  - destruct m' as [ | m'']; cbn; auto.
+    eapply Return_SpecT_con.
+    + eapply Seq_SpecT.
+      eapply LiftTapes_SpecT. smpl_dupfree. cbn. apply Add_SpecT.
+      cbn. intros []. apply LiftTapes_SpecT. smpl_dupfree. cbn. apply MoveValue_SpecT.
+      reflexivity.
+    + cbn. auto.
+  - destruct m' as [ | m'']; cbn; auto.
+    eapply Return_SpecT_con.
+    apply Nop_SpecT. cbn. auto.
+  - intros tin ymid tout HEnc H1.
+    cbn. destruct ymid, m' as [ | m'']; cbn in *; auto.
+    unfold Mult_Step_steps, MoveValue_steps, CaseNat_steps, Add_steps. rewrite !Encode_nat_hasSize. (* Normally, this shouldn't be unfolded here. *)
+    omega.
+Restart.
+  eapply If_SpecT.
+  - hsteps.
+  - destruct m' as [ | m'']; cbn; auto.
+    hsteps. apply Add_SpecT. cbn. hsteps. cbn. apply MoveValue_SpecT. reflexivity. cbn. auto.
+  - destruct m' as [ | m'']; cbn; auto.
+    hsteps. auto.
+  - intros tin ymid tout HEnc H1. (* This part is the same *)
+    cbn. destruct ymid, m' as [ | m'']; cbn in *; auto.
+    unfold Mult_Step_steps, MoveValue_steps, CaseNat_steps, Add_steps. rewrite !Encode_nat_hasSize.
+    omega.
+Qed.
+
+
+Definition Mult_Step_space m' n c : Vector.t (nat->nat) 5 :=
+  match m' with
+  | 0 => [|id; id; id; id; id|]
+  | S m'' => [| (*0*) S;
+               (*1*) Add_space n c @> Fin0; (* = [id] *)
+               (*2*) (Add_space n c @> Fin1) >> MoveValue_size_y (n+c) c;
+               (*3*) (Add_space n c @> Fin2) >> MoveValue_size_x (n+c);
+               (*4*) (Add_space n c @>Fin3) |]
+  end.
+
+Lemma Mult_Step_SpecT_size m' n c ss :
+  TripleT
+    (tspec (withSpace (SpecVector [|Contains _ m'; Contains _ n; Contains _ c; Void; Void|]) ss))
+    (Mult_Step_steps m' n c)
+    (Mult_Step)
+    (fun yout =>
+       tspec
+         (withSpace
+            match yout, m' with
+            | Some _, 0 => SpecVector [|Contains _ m'; Contains _ n; Contains _ c; Void; Void|]
+            | None, S m'' => SpecVector [|Contains _ m''; Contains _ n; Contains _ (n+c); Void; Void|]
+            | _, _ => SpecFalse
+            end (appSize (Mult_Step_space m' n c) ss))).
+Proof.
+  eapply If_SpecT.
+  - hsteps.
+  - destruct m' as [ | m'']; cbn; auto.
+    hsteps. apply Add_SpecT_space. cbn. hsteps. cbn. apply MoveValue_SpecT_size. reflexivity. cbn. auto.
+  - destruct m' as [ | m'']; cbn; auto.
+    hsteps. auto.
+  - intros tin ymid tout HEnc H1. (* This part is the same *)
+    cbn. destruct ymid, m' as [ | m'']; cbn in *; eauto.
+    unfold Mult_Step_steps, MoveValue_steps, CaseNat_steps, Add_steps. rewrite !Encode_nat_hasSize.
+    omega.
+Qed.
+
+
+
+Definition Mult_Loop := While Mult_Step.
+
+Fixpoint Mult_Loop_steps m' n c :=
+  match m' with
+  | O => S (Mult_Step_steps m' n c)
+  | S m'' => S (Mult_Step_steps m' n c) + Mult_Loop_steps m'' n (n + c)
+  end.
+
+
+Lemma Mult_Loop_SpecT m' n c :
+  TripleT
+    (tspec (SpecVector [|Contains _ m'; Contains _ n; Contains _ c; Void; Void|]))
+    (Mult_Loop_steps m' n c)
+    (Mult_Loop)
+    (fun _ => tspec (SpecVector [|Contains _ 0; Contains _ n; Contains _ (m' * n + c); Void; Void|])).
+Proof.
+  eapply While_SpecT with (P := fun '(m',n,c) => _) (R := fun '(m',n,c) => _) (f := fun '(m,n,c) => _) (g := fun '(m,n,c) => _) (x := (m',n,c)); clear m' n c.
+  - intros ((m'&n)&c). apply Mult_Step_SpecT.
+  - intros ((m'&n)&c). cbn. intros _ tmid tout H1 H2. destruct m' as [ | m'']; cbn in *; auto.
+  - intros ((m'&n)&c). cbn. intros tin tmid H1 H2. destruct m' as [ | m'']; cbn in *; auto.
+    eexists (_,_,_). repeat split; eauto.
+    intros _ tout. replace (m'' * n + (n + c)) with (S m'' * n + c) by (ring_simplify; omega). auto.
+Qed.
+
+Fixpoint Mult_Loop_size m' n c :=
+  match m' with
+  | 0 => Mult_Step_space m' n c (* [id;...;id] *)
+  | S m'' => Mult_Step_space m' n c >>> Mult_Loop_size m'' n (n+c)
+  end.
+
+Lemma Mult_Loop_SpecT_size m' n c ss :
+  TripleT
+    (tspec (withSpace (SpecVector [|Contains _ m'; Contains _ n; Contains _ c; Void; Void|]) ss))
+    (Mult_Loop_steps m' n c)
+    (Mult_Loop)
+    (fun _ => tspec (withSpace
+                    (SpecVector [|Contains _ 0; Contains _ n; Contains _ (m' * n + c); Void; Void|])
+                    (appSize (Mult_Loop_size m' n c) ss))).
+Proof.
+  eapply While_SpecT with (P := fun '(m',n,c,ss) => _) (Q := fun '(m',n,c,ss) => _) (R := fun '(m',n,c,ss) => _) (f := fun '(m,n,c,ss) => _) (g := fun '(m,n,c,ss) => _) (x := (m',n,c,ss));
+    clear m' n c ss; intros (((m',n),c),ss).
+  - apply Mult_Step_SpecT_size.
+  - cbn. intros _ tmid tout H1 H2. destruct m' as [ | m'']; cbn in *; auto.
+  - cbn. intros tin tmid H1 H2. destruct m' as [ | m'']; cbn in *; auto.
+    eexists (_,_,_,_). repeat split; eauto.
+    intros _ tout. replace (m'' * n + (n + c)) with (S m'' * n + c) by (ring_simplify; omega). auto.
+Qed.
+
+  
+Definition Mult : pTM sigNat^+ unit 6 :=
+  LiftTapes (CopyValue _) [|Fin0; Fin5|];; (* m' := m *)
+  LiftTapes (Constr_O) [|Fin2|];; (* c := 0 *)
+  LiftTapes Mult_Loop [|Fin5; Fin1; Fin2; Fin3; Fin4|];; (* Main loop *)
+  LiftTapes (Reset _) [|Fin5|]. (* Reset m'=0 *)
+
+
+Definition Mult_steps (m n : nat) : nat := 12 * m + Mult_Loop_steps m n 0 + 57.
+
+
+Lemma Mult_SpecT (m n : nat) :
+  TripleT
+    (tspec (SpecVector [|Contains _ m; Contains _ n; Void; Void; Void; Void|]))
+    (Mult_steps m n)
+    (Mult)
+    (fun _ => tspec (SpecVector [|Contains _ m; Contains _ n; Contains _ (m * n); Void; Void; Void|])).
+Proof.
+  eapply Seq_SpecT.
+  apply LiftTapes_SpecT. smpl_dupfree. apply CopyValue_SpecT.
+  cbn. intros _. eapply Seq_SpecT.
+  apply LiftTapes_SpecT. smpl_dupfree. apply Constr_O_SpecT.
+  cbn. intros _. eapply Seq_SpecT.
+  apply LiftTapes_SpecT. smpl_dupfree. apply Mult_Loop_SpecT.
+  cbn. intros _.
+  eapply LiftTapes_SpecT_con. smpl_dupfree. apply Reset_SpecT.
+  cbn. intros _. replace (m * n + 0) with (m * n) by omega. auto.
+  reflexivity. reflexivity.
+  unfold Mult_steps. ring_simplify. unfold CopyValue_steps, Constr_O_steps, Reset_steps. rewrite !Encode_nat_hasSize. cbn. ring_simplify. reflexivity.
+Restart.
+  unfold Mult. hsteps_cbn.
+  apply CopyValue_SpecT. hsteps_cbn.
+  apply Mult_Loop_SpecT. apply Reset_SpecT.
+  cbn. replace (m * n + 0) with (m * n) by omega. auto. (* This part is the same. *)
+  reflexivity. reflexivity.
+  unfold Mult_steps. ring_simplify. unfold CopyValue_steps, Constr_O_steps, Reset_steps. rewrite !Encode_nat_hasSize. cbn. ring_simplify. reflexivity.
+Qed.
+
+
+
+(** Example for bug-spotting in size functions. *)
+
+Definition Mult_size_bug (m n : nat) : Vector.t (nat->nat) 6 :=
+  [|(*0*) id;
+    (*1*) Mult_Loop_size m n 0 @> Fin1;
+    (*2*) Constr_O_size >> Mult_Loop_size m n 0 @> Fin2;
+    (*3*) Mult_Loop_size m n 0 @> Fin3;
+    (*4*) Mult_Loop_size m n 0 @> Fin4;
+    (*5*) CopyValue_size m >> Mult_Loop_size m n 0 @> Fin4 (* Something wrong here! *)
+   |].
+
+
+Lemma Mult_SpecT_space (m n : nat) (ss : Vector.t nat 6) :
+  TripleT
+    (tspec (withSpace (SpecVector [|Contains _ m; Contains _ n; Void; Void; Void; Void|]) ss))
+    (Mult_steps m n)
+    (Mult)
+    (fun _ => tspec (withSpace (SpecVector [|Contains _ m; Contains _ n; Contains _ (m * n); Void; Void; Void|])
+                            (appSize (Mult_size_bug m n) ss))).
+Proof.
+  unfold Mult.
+  hstep. hstep. cbn. 
+  apply CopyValue_SpecT_size.
+  cbn. intros _. hsteps.
+  cbn. intros _. hstep. cbn. hstep. cbn. apply Mult_Loop_SpecT_size.
+  cbn. intros. hstep. cbn. apply Reset_SpecT_space.
+  cbn. intros _. replace (m * n + 0) with (m * n) by omega.
+  Fail now auto. (** If everything was fine, [auto] would have worked here. We can use [tspec_ext] to find what is wrong. *)
+  tspec_ext. (** Oh! I forgot to add [>> Reset_size 0]. And it should also be [Fin0] instead of [Fin0] *)
+Abort.
+
+
+Definition Mult_size (m n : nat) : Vector.t (nat->nat) 6 :=
+  [|(*0*) id;
+    (*1*) Mult_Loop_size m n 0 @> Fin1;
+    (*2*) Constr_O_size >> Mult_Loop_size m n 0 @> Fin2;
+    (*3*) Mult_Loop_size m n 0 @> Fin3;
+    (*4*) Mult_Loop_size m n 0 @> Fin4;
+    (*5*) CopyValue_size m >> Mult_Loop_size m n 0 @> Fin0 >> Reset_size 0
+   |].
+
+Lemma Mult_SpecT_space (m n : nat) (ss : Vector.t nat 6) :
+  TripleT
+    (tspec (withSpace (SpecVector [|Contains _ m; Contains _ n; Void; Void; Void; Void|]) ss))
+    (Mult_steps m n)
+    (Mult)
+    (fun _ => tspec (withSpace (SpecVector [|Contains _ m; Contains _ n; Contains _ (m * n); Void; Void; Void|])
+                            (appSize (Mult_size m n) ss))).
+Proof.
+  unfold Mult.
+  hstep. hstep. cbn. 
+  apply CopyValue_SpecT_size.
+  cbn. intros _. hsteps.
+  cbn. intros _. hstep. cbn. hstep. cbn. apply Mult_Loop_SpecT_size.
+  cbn. intros. hstep. cbn. apply Reset_SpecT_space.
+  cbn. intros _ t. replace (m * n + 0) with (m * n) by omega. auto. (** Now it is fine! *)
+
+  reflexivity. reflexivity.
+  unfold Mult_steps. ring_simplify. unfold CopyValue_steps, Constr_O_steps, Reset_steps. rewrite !Encode_nat_hasSize. cbn. ring_simplify. reflexivity.
+Qed.
+
+
+(* TODO:
+- Examples using the Sigma-lift
+*)
