theories/TM/Hoare/HoareTactics.v
@@ -1,0 +1,262 @@
+(** ** Very Convienient Verification Tactics for Hoare Logic *)
+
+From Undecidability Require Import ProgrammingTools.
+From Undecidability Require Import TM.Hoare.HoareLogic TM.Hoare.HoareCombinators TM.Hoare.HoareRegister.
+From smpl Require Import Smpl.
+
+(** We define tactics to "execute" the machine step-by-step during the verification. It uses [smpl] to be user-extensible. *)
+
+
+
+(** Checks whether the given term contains an evar *)
+Ltac contains_evar e :=
+  match e with
+  | context [?x] => is_evar x
+  end.
+
+(** Check if the goal triple is with space *)
+Ltac triple_with_space :=
+  lazymatch goal with
+  | [ |- context [withSpace] ] => idtac
+  end.
+
+
+
+(** *** Smpl setup *)
+
+(* For user extensions, like in [TM_Correct] *)
+Smpl Create hstep_smpl.
+Ltac hstep_smpl := smpl hstep_smpl.
+
+
+(** *** Combinators *)
+
+(** There is no tactic for While. *)
+
+
+Ltac hstep_Seq :=
+  match goal with
+  | [ |- Triple ?P (?M1;; ?M2) ?Q ] => eapply Seq_Spec
+  | [ |- TripleT ?P ?k (?M1;; ?M2) ?Q ] => eapply Seq_SpecT
+  end.
+
+(** Note: We often want to specify the running times ([k2] and [k3]) of [M2] and [M3] manually. For that, the user has to apply [If_SpecT] manually. *)
+(** If desired, the user can apply the weak version [If_SpecT_weak] or [If_SpecT_weak'] manually. *)
+Ltac hstep_If :=
+  lazymatch goal with
+  | [ |- Triple ?P (If ?M1 ?M2 ?M3) ?Q ] => eapply If_Spec
+  | [ |- TripleT ?P ?k (If ?M1 ?M2 ?M3) ?Q ] => eapply If_SpecT
+  end.
+
+Ltac hstep_Switch :=
+  lazymatch goal with
+  | [ |- Triple ?P (Switch ?M1 ?M2) ?Q ] => eapply Switch_Spec
+  | [ |- TripleT ?P ?k (Switch ?M1 ?M2) ?Q ] => eapply Switch_SpecT
+  end.
+
+
+(** For [Return], we may have to use the rule [Return_Spec_con]. *)
+Ltac hstep_Return :=
+  lazymatch goal with
+  | [ |- Triple ?P (Return ?M ?x) ?Q ] =>
+    tryif contains_evar Q then (eapply Return_Spec)
+    else (eapply Return_Spec_con)
+  | [ |- TripleT ?P ?k (Return ?M ?x) ?Q ] =>
+    tryif contains_evar Q then (eapply Return_SpecT)
+    else (eapply Return_SpecT_con)
+
+  | [ |- Triple ?P (Relabel ?M ?f) ?Q ] =>
+    tryif contains_evar Q then (eapply Relabel_Spec)
+    else (eapply Relabel_Spec_con)
+  | [ |- TripleT ?P ?k (Relabel ?M ?f) ?Q ] =>
+    tryif contains_evar Q then (eapply Relabel_SpecT)
+    else (eapply Relabel_SpecT_con)
+  end.
+
+
+
+(** ** Lifts *)
+
+(** The rules for the lifts have been implemented for register machines only *)
+(** We have special rules for specifications with space; and we also have to check whether the post-condition already is instantiated. *)
+Ltac hstep_LiftTapes :=
+  lazymatch goal with
+  | [ |- Triple ?P (?M @ ?I) ?Q ] =>
+    tryif contains_evar Q then (* The post-condition is yet to be instantiated. *)
+      (tryif triple_with_space then (eapply LiftTapes_Spec_space; [smpl_dupfree | ])
+        else (eapply LiftTapes_Spec; [smpl_dupfree | ]))
+    else (* Otherwise, we have to use the Consequence rule *)
+      (tryif triple_with_space then (eapply LiftTapes_Spec_space_con; [smpl_dupfree | | ])
+        else (eapply LiftTapes_Spec_con; [smpl_dupfree | | ]))
+  | [ |- TripleT ?P ?k (?M @ ?I) ?Q ] =>
+    tryif contains_evar Q then
+      (tryif triple_with_space then (eapply LiftTapes_SpecT_space; [smpl_dupfree | ])
+        else (eapply LiftTapes_SpecT; [smpl_dupfree | ]))
+    else
+      (tryif triple_with_space then (eapply LiftTapes_SpecT_space_con; [smpl_dupfree | | ])
+        else (eapply LiftTapes_SpecT_con; [smpl_dupfree | | ]))
+  end.
+
+
+(** [ChangeAlphabet] is similar to [LiftTapes], but we always have to apply at least [Consequence_pre]. We also have specialised rules for space. *)
+Ltac hstep_ChangeAlphabet :=
+  lazymatch goal with
+  | [ |- Triple ?P (?M ⇑ ?I) ?Q ] =>
+    tryif contains_evar Q then (* The post-condition is yet to be instantiated. *)
+      (tryif triple_with_space then (eapply ChangeAlphabet_Spec_space_pre; [ | ])
+        else (eapply ChangeAlphabet_Spec_pre; [ | ]))
+    else (* Otherwise, we have to use the Consequence rule *)
+      (tryif triple_with_space then (eapply ChangeAlphabet_Spec_space_pre_post; [ | | ])
+        else (eapply ChangeAlphabet_Spec_pre_post; [ | | ]))
+  | [ |- TripleT ?P ?k (?M ⇑ ?I) ?Q ] =>
+    tryif contains_evar Q then
+      (tryif triple_with_space then (eapply ChangeAlphabet_SpecT_space_pre; [ | ])
+        else (eapply ChangeAlphabet_SpecT_pre; [ | ]))
+    else
+      (tryif triple_with_space then (eapply ChangeAlphabet_SpecT_space_pre_post; [ | | ])
+        else (eapply ChangeAlphabet_SpecT_pre_post; [ | | ]))
+  end.
+
+(*
+Ltac hstep_ChangeAlphabet :=
+  lazymatch goal with
+  | [ |- Triple ?P (?M ⇑ ?I) ?Q ] =>
+    tryif contains_evar Q then (eapply ChangeAlphabet_Spec)
+    else (eapply ChangeAlphabet_Spec_con; [ | ])
+  | [ |- TripleT ?P ?k (?M ⇑ ?I) ?Q ] =>
+    tryif contains_evar Q then (eapply ChangeAlphabet_SpecT)
+    else (eapply ChangeAlphabet_SpecT_pre_post; [ | ])
+  end.
+*)
+
+
+(*
+(** After applying lifts, we have to push [withSpace] to the front of the premise again. *)
+Ltac hstep_withSpace_swap :=
+  lazymatch goal with
+  (** Rule for the tapes lift *)
+  | [ |- Triple  (tspec (Frame (withSpace ?P ?ss) ?I (withSpace ?P' ?ss')))    ?M ?Q ] => eapply Triple_Frame_withSpace;  [now smpl_dupfree | ]
+  | [ |- TripleT (tspec (Frame (withSpace ?P ?ss) ?I (withSpace ?P' ?ss'))) ?k ?M ?Q ] => eapply TripleT_Frame_withSpace; [now smpl_dupfree | ]
+
+  | [ |- Triple  (tspec (Downlift (withSpace ?P ?ss) ?I))    ?M ?Q ] => eapply Triple_Downlift_withSpace
+  | [ |- TripleT (tspec (Downlift (withSpace ?P ?ss) ?I)) ?k ?M ?Q ] => eapply TripleT_Downlift_withSpace
+
+  (** Rules for the alphabet lift *)
+  | [ |- Triple  (tspec (LiftSpec ?I (withSpace ?P ?ss)))    ?M ?Q ] => eapply Triple_LiftSpec_withSpace
+  | [ |- TripleT (tspec (LiftSpec ?I (withSpace ?P ?ss))) ?k ?M ?Q ] => eapply TripleT_LiftSpec_withSpace
+  end.
+*)
+
+
+(** *** Custom machines *)
+
+(** We have to be carefull with [Nop] and custom machines, because usually the postcondition is already instantiated. *)
+
+(** The user only needs to specify the Termination rule. If the user wants to prove partial correctness, it it first checked whether
+there is a corresponding Termination lemma. The tactic also takes care of whether we first have to apply the consequence rule. *)
+
+Ltac hstep_user :=
+  lazymatch goal with
+  | [ |- Triple ?P ?M ?Q ] => (* Without time *)
+    tryif contains_evar Q then
+      (tryif triple_with_space then
+          (* Without time, but with space *)
+          ((eapply TripleT_Triple; hstep_smpl) (* Weaken a registered rule with time and space *)
+           || (hstep_smpl))
+        else ((eapply TripleT_Triple; eapply TripleT_RemoveSpace; now (intros; hstep_smpl)) (* Weaken a registered rule with time and space *)
+              || (eapply Triple_RemoveSpace; now (intros; hstep_smpl)) (* Weaken a registered rule without time but with space *)
+              || (eapply TripleT_Triple; hstep_smpl) (* Weaken a registered rule with time but without space *)
+              || (hstep_smpl))) (* A registered rule without time and without space *)
+    else (eapply Consequence_post; [ hstep_user | ]) (* First apply the consequence rule, then try again *)
+  | [ |- TripleT ?P ?k ?M ?Q ] => (* With time *)
+    tryif contains_evar Q then
+      (tryif triple_with_space then hstep_smpl (* Apply the rule with time and space *)
+        else (eapply TripleT_RemoveSpace; now (intros; hstep_smpl)) (* Weaken a rule with time and space *)
+             || (hstep_smpl))
+    else (eapply ConsequenceT_post; [ hstep_user | ]) (* First apply the consequence rule, then try again *)
+  end.
+
+(** Example: [Nop] *)
+
+Ltac hstep_Nop :=
+  lazymatch goal with
+  (* | [ |- Triple ?P Nop ?Q ] => eapply Nop_Spec *)
+  | [ |- TripleT ?P ?k Nop ?Q ] => eapply Nop_SpecT
+  end.
+
+Smpl Add hstep_Nop : hstep_smpl.
+
+
+(** *** Verification step tactic *)
+
+(** Removes [forall (x : unit] from the goal *)
+Ltac hstep_forall_unit :=
+  lazymatch goal with
+  | [ |- unit -> ?H ] => intros _
+  | [ |- forall (y : finType_CS unit), ?H] => intros [] (* This is usually simplified to the first case with [cbn] *)
+  | [ |- forall (y : unit), ?H] => intros []
+  end.
+
+
+Ltac hstep_Combinators := hstep_Seq || hstep_If || hstep_Switch || hstep_Return. (* Not [While]! *)
+Ltac hstep_Lifts := (hstep_LiftTapes || hstep_ChangeAlphabet).
+Ltac hstep := (*repeat hstep_withSpace_swap;*) (hstep_forall_unit || hstep_Combinators || hstep_Lifts || hstep_user)(*; repeat hstep_withSpace_swap*).
+Ltac hsteps := repeat hstep.
+Ltac hsteps_cbn := repeat (cbn; hstep). (* Calls [cbn] before each verification step *)
+
+
+(** *** More automation for register specifications *)
+
+
+(** Proofs assertions like [tspec (SpecVector ?R) ?t] *)
+Ltac tspec_solve :=
+  lazymatch goal with
+  | [ |- tspec (SpecVector ?R) ?t ] =>
+    eapply tspec_solve; intros i; destruct_fin i;
+    cbn [tspec_single Vector.nth Vector.case0 Vector.caseS]; try (contains_ext || isVoid_mono)
+  | [ |- tspec (withSpace (SpecVector ?R) ?ss) ?t ] => (* We may unfold [withSpace] and simplify now *)
+    eapply tspec_space_solve; intros i; destruct_fin i;
+    cbn [tspec_single withSpace_single Vector.map Vector.nth Vector.case0 Vector.caseS]; try (contains_ext || isVoid_mono)
+  end.
+
+
+(*
+(** Pushes up [withSpace] in [tspec]s *)
+Ltac tspec_withSpace_swap :=
+  lazymatch goal with
+  | [ H : ?t ≃≃ Frame (withSpace ?P ?ss) ?I (withSpace ?P' ?ss') |- _ ] =>
+    apply tspec_Frame_withSpace in H; [ cbn in H; tspec_withSpace_swap |  now smpl_dupfree ]
+  | [ H : ?t ≃≃ Downlift (withSpace ?P ?ss) ?I |- _ ] =>
+    apply tspec_Downlift_withSpace in H; cbn in H; tspec_withSpace_swap
+  | [ H : ?t ≃≃ LiftSpec ?I (withSpace ?P ?ss) |- _ ] =>
+    apply tspec_LiftSpec_withSpace in H; cbn in H; tspec_withSpace_swap
+  | _ => idtac
+end.
+*)
+
+
+(** Proofs assertions like [tspec (SpecVector ?R) ?t] given [tspec (SpecVector ?R') ?t]. Similar to [contains_ext] and [isVoid_mono]. *)
+(** Normally, [eauto] should be able to solve this kind of goal. This tactic helps to find out if there is an error. *)
+Ltac tspec_ext :=
+  (*tspec_withSpace_swap;*)
+  lazymatch goal with
+  | [ |- forall t, t ≃≃ ?P -> t ≃≃ ?Q ] =>
+    let Ht := fresh "H"t in
+    intros t Ht; tspec_ext; eauto
+  | [ H : tspec (SpecVector ?R') ?t |- tspec (SpecVector ?R) ?t ] =>
+    apply tspec_ext with (1 := H);
+    ((now eauto)
+     || (intros i; destruct_fin i;
+        cbn [tspec_single Vector.nth Vector.case0 Vector.caseS];
+        intros; try (contains_ext || isVoid_mono)))
+    | [ H : tspec (withSpace (SpecVector ?R') ?ss) ?t |- tspec (withSpace (SpecVector ?R) ?ss') ?t ] =>
+    apply tspec_space_ext with (1 := H);
+    ((now eauto)
+     || (intros i; destruct_fin i;
+        cbn [tspec_single withSpace_single Vector.nth Vector.case0 Vector.caseS];
+        intros; try (contains_ext || isVoid_mono)))
+  end.
+
+(* (* Maybe not a good idea *)
+Hint Extern 10 => tspec_ext.
+*)
