theories/TM/Single/StepTM.v
@@ -1,11 +1,10 @@
-(* Require Import Combinators.Combinators Multi Basic.Mono TMTac. *)
+(* From Undecidability Require Import Combinators.Combinators Multi Basic.Mono TMTac. *)
 From Undecidability Require Import ProgrammingTools.
 From Undecidability Require Import ArithPrelim.
-
 From Undecidability Require Import TM.Compound.Shift.
 
 From Undecidability Require Import EncodeTapes.
-Require Import FunInd.
+From Coq Require Import FunInd.
 
 
 Local Set Printing Coercions.
